tmp

code/experimental/rsa/Division.fst
@@ -15,75 +15,98 @@ module U64 = FStar.UInt64
 
 type bignum = buffer FStar.UInt64.t
 
+type lbytes (len:U32.t) = 
+     b:buffer FStar.UInt64.t{length b = U32.v len} 
+
+type bnlen = (l:U32.t{U32.v l > 0 /\ U32.v l <= 8192})
+type rem_state (rLen:bnlen) (modLen:bnlen) = lbytes U32.(rLen +^ rLen +^ modLen +^ modLen)
+
+let get_r_i #r #m (st:rem_state r m) : lbytes r = Buffer.sub st 0ul r
+let get_tmp #r #m (st:rem_state r m) : lbytes r = Buffer.sub st r r
+let get_mod #r #m (st:rem_state r m) : lbytes m = Buffer.sub st U32.(r +^ r) m
+let get_mod_1 #r #m (st:rem_state r m) :lbytes m = Buffer.sub st U32.(r +^ r +^ m) m
+
+let rem_state_inv r m (st:rem_state r m) = 
+           let r_i = get_r_i st in
+           let tmp = get_tmp st in
+           let mod = get_mod st in
+           let mod_1 = get_mod_1 st in
+           let r = frameOf r_i in
+	     r == frameOf mod /\
+	     r == frameOf mod_1 /\
+	     r == frameOf tmp /\
+	     disjoint r_i tmp /\
+	     disjoint r_i mod /\
+	     disjoint r_i mod_1 /\ 
+	     disjoint tmp mod /\ 
+	     disjoint tmp mod_1 /\ 
+       	     disjoint mod mod_1 
+
+
+let rem_state_st_inv (rLen:bnlen) (modLen:bnlen) (st:rem_state rLen modLen) (h:FStar.HyperStack.mem) = 
+	     rem_state_inv rLen modLen st /\ live h st
+		       
+
 [@ "substitute"]
 val remainder_r_i:
-    rLen:U32.t{U32.v rLen > 0} ->
-    modLen:U32.t{U32.v modLen > 0 /\ U32.v modLen = U32.v rLen} ->
-    r_i:bignum{length r_i = U32.v rLen} ->
-    mod:bignum{length mod = U32.v modLen /\ disjoint r_i mod} ->
-    tmp_b:bool -> Stack unit
-    (requires (fun h -> live h r_i /\ live h mod))
-	(ensures (fun h0 _ h1 -> live h0 r_i /\ live h0 mod /\
-        live h1 r_i /\ live h1 mod /\ modifies_1 r_i h0 h1))
+    rLen:bnlen -> modLen:bnlen{U32.v modLen = U32.v rLen} ->
+    tmp_b:bool -> st:rem_state rLen modLen -> Stack unit 
+    	       (requires (fun h -> rem_state_st_inv rLen modLen st h))
+	       (ensures (fun h r h' -> rem_state_st_inv rLen modLen st h' /\
+				     modifies_1 st h h'))
+let remainder_r_i rLen modLen tmp_b st =
+    if not tmp_b then
+	let r_i = get_r_i st in
+	let tmp = get_tmp st in
+	let mod = get_mod st in
+        sub rLen modLen r_i mod tmp;
+        blit tmp 0ul r_i 0ul rLen
 
-let remainder_r_i rLen modLen r_i mod tmp_b =
-    push_frame();
-    let tmp = create 0uL rLen in
-    let h0 = ST.get () in
-    (if not tmp_b then
-        (sub rLen modLen r_i mod tmp;
-        blit tmp 0ul r_i 0ul rLen));
-    lemma_modifies_sub_1 h0 h0 r_i;
-    pop_frame()
+let lemma_modifies_0_is_modifies_1 (#a:Type) (h:HyperStack.mem) (b:buffer a{live h b}) : Lemma
+  (modifies_1 b h h) =
+  lemma_modifies_sub_1 h h b
 
-// BB. TODO
-let lemma_modifies_1_0_1_1_is_modifies_3 #t h0 h1 h1' h1'' h2 h3 (b0:buffer t) (b1:buffer t{disjoint b1 b0}) (b2:buffer t{disjoint b2 b0 /\ disjoint b2 b1}) : Lemma
-  (requires (modifies_1 b0 h0 h1 /\ h1 == h1' /\ modifies_0 h1' h1'' /\ modifies_1 b1 h1'' h2 /\ modifies_1 b2 h2 h3))
-  (ensures  (modifies_3 b0 b1 b2 h0 h3))
-  = admit()
-
-// BB. TODO
-let lemma_modifies_1_is_modifies_3 #t h0 h1 h2 (b0:buffer t) (b1:buffer t{disjoint b1 b0}) (b2:buffer t{disjoint b2 b0 /\ disjoint b2 b1}) : Lemma
-  (requires (modifies_1 b0 h0 h1 /\ modifies_0 h1 h2))
-  (ensures  (modifies_3 b0 b1 b2 h0 h2))
-  = admit()
 
 
 val remainder_loop:
-    rLen:U32.t{U32.v rLen > 0} ->
-    modLen:U32.t{U32.v modLen > 0 /\ U32.v modLen = U32.v rLen} ->
-    r_i:bignum{length r_i = U32.v rLen} ->
-    mod:bignum{length mod = U32.v modLen /\ disjoint r_i mod} ->
-    mod1:bignum{length mod1 = U32.v modLen /\ disjoint mod mod1 /\ disjoint r_i mod1} ->
-    count:U32.t -> Stack unit
-    (requires (fun h -> live h r_i /\ live h mod /\ live h mod1))
-	(ensures (fun h0 _ h1 -> live h0 r_i /\ live h0 mod /\ live h0 mod1 /\
-        live h1 r_i /\ live h1 mod /\ live h1 mod1 /\ modifies_3 mod1 r_i mod h0 h1))
+    rLen:bnlen -> modLen:bnlen{ U32.v modLen = U32.v rLen} ->
+    count:U32.t ->  st:rem_state rLen modLen -> Stack unit
+    (requires (fun h -> rem_state_st_inv rLen modLen st h))
+    (ensures (fun h0 _ h1 -> rem_state_st_inv rLen modLen st h1 /\ 
+			   modifies_1 st h0 h1))
 
-#set-options "--z3rlimit 150 --max_fuel 1"
-
-let rec remainder_loop rLen modLen r_i mod mod1 count =
-  (**) let h0 = ST.get () in
-  rshift1 modLen mod mod1;
-  (**) let h1 = ST.get () in
+#set-options "--z3rlimit 300 --max_fuel 0"
+let rec remainder_loop rLen modLen count st =
   if U32.(count >^ 0ul) then begin
-    (**) assert(modifies_1 mod1 h0 h1);
-    (**) let h1' = ST.get () in
+    let tmp = get_tmp st in
+    let mod_1 = get_mod_1 st in
+    let r_i = get_r_i st in
+    let mod = get_mod st in
+    let h1 = ST.get() in
     let tmp_b = isMore modLen rLen mod r_i in
-    (**) let h1'' = ST.get () in
-    remainder_r_i rLen modLen r_i mod tmp_b;
-    (**) let h2 = ST.get () in
-    blit mod1 0ul mod 0ul modLen;
-    (**) let h3 = ST.get () in
-    (**) lemma_modifies_1_0_1_1_is_modifies_3 h0 h1 h1' h1'' h2 h3 mod1 r_i mod;
-    (**) assert(modifies_3 mod1 r_i mod h0 h3);
-    remainder_loop rLen modLen r_i mod mod1 U32.(count -^ 1ul)
-    end else begin
-    (**) let h3' = ST.get () in
-    (**) lemma_modifies_1_is_modifies_3 h0 h1 h3' mod1 r_i mod;
-    (**) assert(modifies_3 mod1 r_i mod h0 h3')
-    end
+    let h2 = ST.get() in
+    no_upd_lemma_0 h1 h2 st;
+    lemma_modifies_0_is_modifies_1 h2 st; (* IDIOTIC LEMMA NEEDED *)
+    rshift1 modLen mod mod_1;
+    remainder_r_i rLen modLen tmp_b st;
+    blit mod_1 0ul mod 0ul modLen;
+    remainder_loop rLen modLen U32.(count -^ 1ul) st 
+    end 
+    
 
+
+val remainder_:
+    rLen:bnlen ->  modLen:bnlen{U32.v modLen = U32.v rLen} ->
+    count:U32.t ->  st:rem_state rLen modLen -> Stack unit
+    (requires (fun h -> rem_state_st_inv rLen modLen st h))
+    (ensures (fun h0 _ h1 -> rem_state_st_inv rLen modLen st h1 /\ 
+			   modifies_1 st h0 h1))
+
+let remainder_ rLen modLen count st =
+    remainder_loop rLen modLen count st
+
+
+(*
 (* res = a % mod *)
 val remainder:
     aBits:U32.t{U32.v aBits > 0} ->
@@ -119,7 +142,7 @@ let remainder aBits modBits resLen a mod res =
     let r_0 = create 0uL a1Len in
     blit a 0ul r_0 1ul aLen;
 
-    let mod1_tmp = create 0uL modLen in
-    remainder_loop a1Len mod1Len r_0 mod1 mod1_tmp k;
+    remainder_ a1Len mod1Len r_0 mod1 k;
     blit r_0 0ul res 0ul resLen;
     pop_frame()
+    *)
